src/MachineWordStdpp.v
@@ -1,18 +1,80 @@
-From Sail Require MachineWordInterface.
+From Sail Require TypeCasts MachineWordInterface.
 From stdpp Require Import base bitvector.definitions.
 Require Import ZArith.
 Require Import String.
 
 Module MachineWord <: MachineWordInterface.MachineWordInterface.
 
-Definition word n := bv (N.of_nat n).
+Definition idx := N.
 
-Definition zeros n : word n := bv_0 (N.of_nat n).
+Definition Z_idx := Z.to_N.
+Definition N_idx (n : N) := n.
+Definition nat_idx := N.of_nat.
+Hint Unfold Z_idx N_idx nat_idx : core.
+Arguments Z_idx /.
+Arguments N_idx /.
+Arguments nat_idx /.
 
-Definition get_bit [n] (w : word n) i : bool := Z.testbit (bv_unsigned w) (Z.of_nat i).
+Definition idx_Z := Z.of_N.
+Definition idx_N (n : N) := n.
+Definition idx_nat := N.to_nat.
+Arguments idx_Z /.
+Arguments idx_N /.
+Arguments idx_nat /.
 
-Lemma get_bit_eq : forall [n] (w v : word n),
-  (forall i, i < n -> get_bit w i = get_bit v i) -> w = v.
+Lemma Z_idx_Z n : n = Z_idx (idx_Z n).
+Proof.
+  simpl.
+  rewrite N2Z.id.
+  reflexivity.
+Qed.
+Lemma idx_Z_idx z : (z >= 0)%Z -> idx_Z (Z_idx z) = z.
+Proof.
+  intro GE.
+  simpl.
+  rewrite Z2N.id; auto with zarith.
+Qed.
+Lemma nat_idx_Z n : nat_idx n = Z_idx (Z.of_nat n).
+Proof.
+  simpl.
+  rewrite <- Z_nat_N.
+  rewrite Nat2Z.id.
+  reflexivity.
+Qed.
+Lemma idx_N_Z_idx z : idx_N (Z_idx z) = Z.to_N z.
+Proof.
+  simpl.
+  reflexivity.
+Qed.
+
+Definition cast_idx {T m n} := @TypeCasts.cast_N T m n.
+Lemma cast_idx_refl n T (x : T n) (e : n = n) : cast_idx x e = x.
+Proof.
+  apply TypeCasts.cast_N_refl.
+Qed.
+
+Definition idx_S := N.succ.
+Definition idx_add := N.add.
+Definition idx_mul := N.mul.
+Hint Unfold idx_S idx_add idx_mul : core.
+Arguments idx_S /.
+Arguments idx_add /.
+Arguments idx_mul /.
+Lemma Z_idx_S z : (z >= 0)%Z -> Z_idx (Z.succ z) = idx_S (Z_idx z).
+Proof.
+  simpl.
+  intro GE.
+  apply Z2N.inj_succ; lia.
+Qed.
+
+Definition word := bv.
+
+Definition zeros n : word n := bv_0 n.
+
+Definition get_bit [n] (w : word n) i : bool := Z.testbit (bv_unsigned w) (Z.of_N i).
+
+Lemma get_bit_eq_nat : forall [n] (w v : word (nat_idx n)),
+  (forall i, i < n -> get_bit w (nat_idx i) = get_bit v (nat_idx i)) -> w = v.
 intros n w v H.
 apply bv_eq.
 unfold get_bit in *.
@@ -20,9 +82,11 @@ apply Z.bits_inj'.
 intros m LE.
 destruct (Z_lt_dec m (Z.of_nat n)).
 * rewrite <- (Z2Nat.id m LE).
+  rewrite <- nat_N_Z.
   apply H.
   Lia.lia.
-* rewrite !bv_unsigned_spec_high; auto; Lia.lia.
+* unfold nat_idx in *.
+  rewrite !bv_unsigned_spec_high; auto; Lia.lia.
 Qed.
 
 Definition word_to_Z [n] (w : word n) : Z := bv_signed w.
@@ -30,42 +94,44 @@ Definition word_to_N [n] (w : word n) : N := Z.to_N (bv_unsigned w).
 Definition Z_to_word n z : word n := Z_to_bv _ z.
 Definition N_to_word n nn : word n := Z_to_bv _ (Z.of_N nn).
 
-Lemma word_to_N_range : forall [n] (w : word n), (word_to_N w < 2 ^ N.of_nat n)%N.
+Lemma word_to_N_range : forall [n] (w : word n), (word_to_N w < 2 ^ idx_N n)%N.
+unfold idx_N.
 intros.
 specialize (bv_unsigned_in_range _ w).
 unfold bv_modulus.
 intros [LE LT].
 
 unfold word_to_N.
-rewrite <- (N2Z.id (2 ^ N.of_nat n)).
+rewrite <- (N2Z.id (2 ^ n)).
 rewrite <- Z2N.inj_lt;  Lia.lia.
 Qed.
 
 (* TODO: this proof is generic, should be shared *)
-Lemma testbit_word_to_N_high : forall [n] (w: word n) i, (i >= N.of_nat n)%N ->
+Lemma testbit_word_to_N_high : forall [n] (w: word n) i, (i >= n)%N ->
   N.testbit (word_to_N w) i = false.
 intros.
 specialize (word_to_N_range w).
 generalize (word_to_N w) as m.
+unfold idx_N.
 intros.
 destruct (N.testbit_spec m i) as [l [h [H1 H2]]].
 destruct (N.testbit m i).
 * simpl (N.b2n true) in H2. subst.
   assert (l + (1 + 2 * h) * 2 ^ i >= 2 ^ i)%N by Lia.lia.
-  specialize (N.pow_le_mono_r 2 (N.of_nat n) i).
+  specialize (N.pow_le_mono_r 2 n i).
   Lia.lia.
 * reflexivity.
 Qed.
 
-Lemma word_to_Z_range : forall [n] (w : word (S n)), (- 2 ^ Z.of_nat n <= word_to_Z w < 2 ^ Z.of_nat n)%Z.
+Lemma word_to_Z_range : forall [n] (w : word (N.succ n)), (- 2 ^ idx_Z n <= word_to_Z w < 2 ^ idx_Z n)%Z.
+unfold idx_Z.
 intros.
 specialize (bv_signed_in_range _ w ltac:(Lia.lia)).
 unfold bv_half_modulus, bv_modulus, word_to_Z.
-rewrite nat_N_Z.
-rewrite Nat2Z.inj_succ.
+rewrite N2Z.inj_succ.
 rewrite Z.pow_succ_r; auto with zarith.
 
-replace (2 * 2 ^ Z.of_nat n / 2)%Z with (2 ^ Z.of_nat n)%Z. 2: {
+replace (2 * 2 ^ Z.of_N n / 2)%Z with (2 ^ Z.of_N n)%Z. 2: {
   rewrite Z.mul_comm.
   rewrite Z.div_mul; auto.
 }
@@ -75,14 +141,15 @@ Qed.
 Definition ones n : word n := Z_to_bv _ (-1).
 
 Definition word_to_bools [n] (w : word n) : list bool := List.rev (bv_to_bits w).
-Definition bools_to_word (l : list bool) : word (List.length l) := N_to_word (List.length l) (Ascii.N_of_digits (List.rev l)).
+Definition bools_to_word (l : list bool) : word (nat_idx (List.length l)) := N_to_word (N.of_nat (List.length l)) (Ascii.N_of_digits (List.rev l)).
 
-Lemma word_to_bools_length : forall [n] (w : word n), List.length (word_to_bools w) = n.
+Lemma word_to_bools_length : forall [n] (w : word n), List.length (word_to_bools w) = idx_nat n.
 intros.
+unfold idx_nat.
 unfold word_to_bools.
 rewrite List.rev_length.
 rewrite bv_to_bits_length.
-apply Nnat.Nat2N.id.
+reflexivity.
 Qed.
 
 Lemma nth_error_lookup {A} (l : list A) (i : nat) :
@@ -119,28 +186,29 @@ destruct (lt_dec i (List.length l)) as [H|H].
 Qed.
 
 Lemma word_to_bools_get_bit : forall [n] (w : word n) (i : nat) x,
-  List.nth_error (word_to_bools w) i = Some x <-> get_bit w (n - i - 1) = x /\ i < n.
+  List.nth_error (word_to_bools w) i = Some x <-> get_bit w (nat_idx (idx_nat n - i - 1)) = x /\ i < idx_nat n.
+unfold nat_idx, idx_nat.
 intros.
 unfold word_to_bools, get_bit.
-specialize (bv_to_bits_lookup_Some w (n - i - 1) x).
+specialize (bv_to_bits_lookup_Some w (N.to_nat n - i - 1) x).
 rewrite nth_error_lookup.
 intro H.
 rewrite nth_error_rev.
 rewrite List.rev_involutive, List.rev_length.
 rewrite bv_to_bits_length.
-rewrite Nnat.Nat2N.id in *.
 rewrite H.
+rewrite nat_N_Z.
 firstorder.
 Lia.lia.
 Qed.
 
-Lemma word_to_bools_nth_Some : forall [n] (w : word n) (i : nat) x, n > 0 ->
-  List.nth_error (word_to_bools w) i = Some x <-> x = N.testbit (word_to_N w) (N.of_nat (n - i - 1)) /\ i < n.
+Lemma word_to_bools_nth_Some : forall [n] (w : word n) (i : nat) x, idx_nat n > 0 ->
+  List.nth_error (word_to_bools w) i = Some x <-> x = N.testbit (word_to_N w) (N.of_nat (idx_nat n - i - 1)) /\ i < idx_nat n.
+unfold idx_nat.
 intros.
 rewrite word_to_bools_get_bit.
 unfold get_bit, word_to_N.
 rewrite <- (Z2N.id (bv_unsigned w)) at 1.
-rewrite <- nat_N_Z.
 rewrite Z.testbit_of_N.
 intuition.
 firstorder using bv_unsigned_in_range.
@@ -181,7 +249,8 @@ induction l.
 Qed.
 
 Lemma bools_to_word_get_bit : forall l i b,
-  List.nth_error l i = Some b <-> get_bit (bools_to_word l) (List.length l - i - 1) = b /\ i < List.length l.
+  List.nth_error l i = Some b <-> get_bit (bools_to_word l) (nat_idx (List.length l - i - 1)) = b /\ i < List.length l.
+unfold nat_idx.
 intros.
 unfold bools_to_word, get_bit, N_to_word.
 rewrite Z_to_bv_unsigned.
@@ -192,7 +261,6 @@ rewrite bv_wrap_small. 2: {
   rewrite List.rev_length.
   Lia.lia.
 }
-erewrite <- nat_N_Z.
 rewrite Z.testbit_of_N.
 rewrite nth_error_rev.
 specialize (nth_error_N_of_digits (List.rev l) (List.length l - i - 1) b).
@@ -210,16 +278,15 @@ rewrite <- (Z2N.id (bv_unsigned (bools_to_word l))) at 1. 2: {
   specialize (bv_unsigned_in_range _ (bools_to_word l)).
   intuition.
 }
-rewrite <- nat_N_Z.
 rewrite Z.testbit_of_N.
 intuition.
 Qed.
 
-Definition slice {m} n (w : word m) i : word n := bv_extract (N.of_nat i) _ w.
+Definition slice {m} n (w : word m) i : word n := bv_extract i _ w.
 Definition update_slice {m n} (w : word m) i (v : word n) : word m :=
-  bv_concat (N.of_nat m)
+  bv_concat m
     (slice (m - n - i) w (i + n))
-    (bv_concat (N.of_nat (i+n)) v (slice i w 0)).
+    (bv_concat (i+n) v (slice i w 0)).
 Definition zero_extend {m} n (w : word m) : word n := bv_zero_extend _ w.
 Definition sign_extend {m} n (w : word m) : word n := bv_sign_extend _ w.
 Definition concat {m n} (w : word m) (v : word n) : word (m + n) := bv_concat _ w v.
@@ -235,11 +302,11 @@ Definition add [n] (w v : word n) : word n := bv_add w v.
 Definition sub [n] (w v : word n) : word n := bv_sub w v.
 Definition mul [n] (w v : word n) : word n := bv_mul w v.
 
-Definition logical_shift_left  [n] (w : word n) i : word n := bv_shiftl w (N_to_word n (N.of_nat i)).
-Definition logical_shift_right [n] (w : word n) i : word n := bv_shiftr w (N_to_word n (N.of_nat i)).
-Definition arith_shift_right   [n] (w : word n) i : word n := bv_ashiftr w (N_to_word n (N.of_nat i)).
+Definition logical_shift_left  [n] (w : word n) i : word n := bv_shiftl w (N_to_word n i).
+Definition logical_shift_right [n] (w : word n) i : word n := bv_shiftr w (N_to_word n i).
+Definition arith_shift_right   [n] (w : word n) i : word n := bv_ashiftr w (N_to_word n i).
 
-Fixpoint replicate m [n] (w : word n) : word (m * n) :=
+Fixpoint replicate m [n] (w : word n) : word (N.of_nat m * n) :=
   match m with
   | O => bv_0 0
   | S m' => bv_concat _ w (replicate m' w)
@@ -254,7 +321,7 @@ destruct (eq_dec w v); split; congruence.
 Qed.
 
 Definition reverse_endian [n] (w : word n) : word n :=
-  let bytes := bv_to_little_endian (Z.div (Z.of_nat n) 8) 8 (bv_unsigned w) in
+  let bytes := bv_to_little_endian (Z.div (Z.of_N n) 8) 8 (bv_unsigned w) in
   Z_to_word n (little_endian_to_bv 8 (List.rev bytes)).
 
 Definition word_to_binary_string [n] (w : word n) : String.string :=
