src/MachineWordInterface.v
@@ -2,45 +2,72 @@ Require Import ZArith.
 
 Module Type MachineWordInterface.
 
-Parameter word : nat -> Type.
+(* The underlying library's type of indices / sizes for bitvectors. *)
+Parameter idx : Type.
+
+Parameter Z_idx : Z -> idx.
+Parameter N_idx : N -> idx.
+Parameter nat_idx : nat -> idx.
+
+Parameter idx_Z : idx -> Z.
+Parameter idx_N : idx -> N.
+Parameter idx_nat : idx -> nat.
+
+(* Enough theory about them to define the rest of the Sail library *)
+Axiom Z_idx_Z : forall n, n = Z_idx (idx_Z n).
+Axiom idx_Z_idx : forall z, (z >= 0)%Z -> idx_Z (Z_idx z) = z.
+Axiom nat_idx_Z : forall n, nat_idx n = Z_idx (Z.of_nat n).
+Axiom idx_N_Z_idx : forall z, idx_N (Z_idx z) = Z.to_N z.
+
+Parameter cast_idx : forall {T : idx -> Type} {m n : idx}, T m -> m = n -> T n.
+Axiom cast_idx_refl : forall n T (x : T n) (e : n = n), cast_idx x e = x.
+
+Parameter idx_S : idx -> idx.
+Parameter idx_add : idx -> idx -> idx.
+Parameter idx_mul : idx -> idx -> idx.
+Axiom Z_idx_S : forall z, (z >= 0)%Z -> Z_idx (Z.succ z) = idx_S (Z_idx z).
+
+(* Now the actual bitvectors. *)
+
+Parameter word : idx -> Type.
 Parameter zeros : forall n, word n.
 Parameter ones : forall n, word n.
-Parameter get_bit : forall [n], word n -> nat -> bool.
-Parameter set_bit : forall [n], word n -> nat -> bool -> word n.
+Parameter get_bit : forall [n], word n -> idx -> bool.
+Parameter set_bit : forall [n], word n -> idx -> bool -> word n.
 
-Axiom get_bit_eq : forall [n] (w v : word n),
-  (forall i, i < n -> get_bit w i = get_bit v i) -> w = v.
+Axiom get_bit_eq_nat : forall [n] (w v : word (nat_idx n)),
+  (forall i, i < n -> get_bit w (nat_idx i) = get_bit v (nat_idx i)) -> w = v.
 
 (* These are big-endian, in keeping with the Lem backend. *)
 Parameter word_to_bools : forall [n], word n -> list bool.
-Parameter bools_to_word : forall l : list bool, word (List.length l).
+Parameter bools_to_word : forall l : list bool, word (nat_idx (List.length l)).
 
 Parameter word_to_Z : forall [n], word n -> Z.
 Parameter word_to_N : forall [n], word n -> N.
 Parameter Z_to_word : forall n, Z -> word n.
 Parameter N_to_word : forall n, N -> word n.
 
-Axiom word_to_N_range : forall [n] (w : word n), (word_to_N w < 2 ^ N.of_nat n)%N.
-Axiom word_to_Z_range : forall [n] (w : word (S n)), (- 2 ^ Z.of_nat n <= word_to_Z w < 2 ^ Z.of_nat n)%Z.
-Axiom testbit_word_to_N_high : forall [n] (w: word n) i, (i >= N.of_nat n)%N ->
+Axiom word_to_N_range : forall [n] (w : word n), (word_to_N w < 2 ^ idx_N n)%N.
+Axiom word_to_Z_range : forall [n] (w : word (idx_S n)), (- 2 ^ idx_Z n <= word_to_Z w < 2 ^ idx_Z n)%Z.
+Axiom testbit_word_to_N_high : forall [n] (w: word n) i, (i >= idx_N n)%N ->
   N.testbit (word_to_N w) i = false.
 
-Axiom word_to_bools_length : forall [n] (w : word n), List.length (word_to_bools w) = n.
+Axiom word_to_bools_length : forall [n] (w : word n), List.length (word_to_bools w) = idx_nat n.
 Axiom word_to_bools_get_bit : forall [n] (w : word n) (i : nat) x,
-  List.nth_error (word_to_bools w) i = Some x <-> get_bit w (n - i - 1) = x /\ i < n.
-Axiom word_to_bools_nth_Some : forall [n] (w : word n) (i : nat) x, n > 0 ->
-  List.nth_error (word_to_bools w) i = Some x <-> x = N.testbit (word_to_N w) (N.of_nat (n - i - 1)) /\ i < n.
+  List.nth_error (word_to_bools w) i = Some x <-> get_bit w (nat_idx (idx_nat n - i - 1)) = x /\ i < idx_nat n.
+Axiom word_to_bools_nth_Some : forall [n] (w : word n) (i : nat) x, idx_nat n > 0 ->
+  List.nth_error (word_to_bools w) i = Some x <-> x = N.testbit (word_to_N w) (N.of_nat (idx_nat n - i - 1)) /\ i < idx_nat n.
 Axiom bools_to_word_get_bit : forall l i b,
-  List.nth_error l i = Some b <-> get_bit (bools_to_word l) (length l - i - 1) = b /\ i < length l.
+  List.nth_error l i = Some b <-> get_bit (bools_to_word l) (nat_idx (length l - i - 1)) = b /\ i < length l.
 Axiom bools_to_word_nth_Some : forall (l : list bool) i b,
   List.nth_error l i = Some b <-> b = N.testbit (word_to_N (bools_to_word l)) (N.of_nat (length l - i - 1)) /\ i < length l.
 
 
-Parameter slice : forall [m] n, word m -> nat -> word n.
-Parameter update_slice : forall [m] [n], word m -> nat -> word n -> word m.
+Parameter slice : forall [m] n, word m -> idx -> word n.
+Parameter update_slice : forall [m] [n], word m -> idx -> word n -> word m.
 Parameter zero_extend : forall [m] n, word m -> word n.
 Parameter sign_extend : forall [m] n, word m -> word n.
-Parameter concat : forall [m] [n], word m -> word n -> word (m + n).
+Parameter concat : forall [m] [n], word m -> word n -> word (idx_add m n).
 
 Parameter and : forall [n], word n -> word n -> word n.
 Parameter  or : forall [n], word n -> word n -> word n.
@@ -51,11 +78,11 @@ Parameter add : forall [n], word n -> word n -> word n.
 Parameter sub : forall [n], word n -> word n -> word n.
 Parameter mul : forall [n], word n -> word n -> word n.
 
-Parameter logical_shift_left  : forall [n], word n -> nat -> word n.
-Parameter logical_shift_right : forall [n], word n -> nat -> word n.
-Parameter arith_shift_right  : forall [n], word n -> nat -> word n.
+Parameter logical_shift_left  : forall [n], word n -> idx -> word n.
+Parameter logical_shift_right : forall [n], word n -> idx -> word n.
+Parameter arith_shift_right  : forall [n], word n -> idx -> word n.
 
-Parameter replicate : forall m [n], word n -> word (m * n).
+Parameter replicate : forall m [n], word n -> word (idx_mul (nat_idx m) n).
 
 Parameter eqb : forall [n], word n -> word n -> bool.
 Axiom eqb_true_iff : forall {n} (w v : word n), eqb w v = true <-> w = v.
